Fix LZ77 specifications.

code/Yazi.LZ77.fst
@@ -57,32 +57,28 @@ assume val hash:
 [@@ CMacro ]
 let min_match = 4ul
 
-[@@ CInline ]
+#set-options "--z3rlimit 2048 --fuel 0 --ifuel 0 --z3refresh"
 inline_for_extraction
-let clear_hash (ctx: lz77_context_p):
-  ST.StackInline unit
-  (requires fun h -> S.context_valid h ctx)
-  (ensures fun h0 _ h1 ->
-    S.context_valid h1 ctx /\
-    B.modifies (B.loc_buffer (B.get h1 (CB.as_mbuf ctx) 0).head) h0 h1 /\
-    S.hash_chain_valid h1 ctx 0ul false) =
-  let head = (CB.index ctx 0ul).head in
-  let h_size = (CB.index ctx 0ul).h_size in
-  B.fill head 0us h_size
-
-#set-options "--z3rlimit 2048 --fuel 0 --ifuel 0"
-inline_for_extraction
-let insert_hash (ctx: lz77_context_p) (state: Ghost.erased lz77_state_t) (i: U32.t):
+let insert_hash (ctx: lz77_context_p) (state: lz77_state_t) (i: U32.t):
   ST.Stack unit
   (requires fun h ->
     let state' = B.as_seq h state in
     S.state_valid h ctx state /\
-    U32.v i <= S.strstart state' + S.lookahead state' - S.min_match /\
-    S.hash_chain_valid h ctx i false)
+    S.insert state' > 0 /\
+    U32.v i <= S.window_end state' - S.min_match /\
+    U32.v i == S.hash_end state' /\
+    S.hash_chain_valid h ctx state false)
   (ensures fun h0 _ h1 ->
-    B.modifies (S.hash_loc_buffer h0 ctx) h0 h1 /\
+    let s0 = B.as_seq h0 state in
+    let s1 = B.as_seq h1 state in
+    S.state_valid h0 ctx state /\
+    B.modifies (
+      S.hash_loc_buffer h0 ctx `B.loc_union`
+      B.loc_buffer state) h0 h1 /\
     S.state_valid h1 ctx state /\
-    S.hash_chain_valid h1 ctx (U32.add i 1ul) false) =
+    LB.unchange_except h0 h1 state 6 /\
+    S.insert s0 - 1 == S.insert s1 /\
+    S.hash_chain_valid h1 ctx state false) =
   let open U32 in
   let head = (CB.index ctx 0ul).head in
   let prev = (CB.index ctx 0ul).prev in
@@ -94,13 +90,14 @@ let insert_hash (ctx: lz77_context_p) (state: Ghost.erased lz77_state_t) (i: U32
   S.window_index_upper_bound h0 ctx (v i);
   S.window_mask_aux (U16.v ctx'.w_bits) (v ctx'.w_size) (U16.v ctx'.w_mask) (v i);
   
-  if CFlags.fastest then begin
+  if CFlags.fastest then
     head.(h) <- Cast.uint32_to_uint16 i
-  end else begin
+  else begin
     UInt.logand_mask (v i) (U16.v ctx'.w_bits);
     prev.(i &^ Cast.uint16_to_uint32 w_mask) <- head.(h);
     head.(h) <- Cast.uint32_to_uint16 i
-  end
+  end;
+  decr_insert state
 
 [@@ CInline ]
 let rec do_init_input_hash
@@ -115,7 +112,6 @@ let rec do_init_input_hash
   (decreases U32.v lookahead + insert) =
   let open U32 in
   insert_hash ctx state i;
-  decr_insert state;
 
   let insert = get_insert state in
   if (lookahead +^ insert <^ min_match) || (insert = 0ul) then
@@ -123,12 +119,7 @@ let rec do_init_input_hash
   else
     do_init_input_hash ctx state (i +^ 1ul) lookahead (U32.v insert)
 
-[@@ CInline ]
-inline_for_extraction
-let init_input_hash (ctx: lz77_context_p) (state: lz77_state_t):
-  ST.Stack unit
-  (requires fun h -> S.init_input_hash_pre h ctx state)
-  (ensures fun h0 _ h1 -> S.init_input_hash_post h0 h1 ctx state) =
+let init_input_hash ctx state =
   let open U32 in
   let lookahead = get_lookahead state in
   let insert = get_insert state in
@@ -137,46 +128,32 @@ let init_input_hash (ctx: lz77_context_p) (state: lz77_state_t):
   else
     ()
 
-[@@ CInline ]
-let rec do_init_dict_hash (ctx: lz77_context_p) (state: lz77_state_t) (i h_end: U32.t):
-  ST.Stack unit
-  (requires fun h -> S.do_init_dict_hash_pre h ctx state i (U32.v h_end))
-  (ensures fun h0 _ h1 -> S.do_init_dict_hash_post h0 h1 ctx state) =
-  let open U32 in
-  insert_hash ctx state i;
-  if i +^ 1ul <^ h_end then
-    do_init_dict_hash ctx state (i +^ 1ul) h_end
-  else
-    ()
-
-let init_dict_hash ctx state =
-  let open U32 in
-  do_init_dict_hash ctx state
-    (get_strstart state)
-    (get_strstart state +^ get_lookahead state -^ (min_match -^ 1ul))
-
 inline_for_extraction let read_buf 
   (ss: stream_state_t)
   (block_data: Ghost.erased (Seq.seq U8.t))
+  (window: B.buffer U8.t)
+  (window_size: Ghost.erased U32.t)
   (next_in: input_buffer)
-  (buf: B.buffer U8.t)
-  (size: U32.t)
+  (from size: U32.t)
   (wrap: wrap_t):
-  ST.Stack (U32.t & Ghost.erased (CB.const_buffer U8.t))
-  (requires fun h -> SS.read_buf_pre h ss block_data next_in buf size wrap)
-  (ensures fun h0 res h1 -> SS.read_buf_post h0 res h1 ss block_data next_in buf size wrap) =
+  ST.Stack (U32.t & Ghost.erased (Seq.seq U8.t))
+  (requires fun h ->
+    SS.read_buf_pre h ss block_data window next_in window_size from size wrap)
+  (ensures fun h0 res h1 ->
+    SS.read_buf_post h0 res h1 ss block_data window next_in window_size from size wrap) =
   let open U32 in
+  let h0 = Ghost.hide (ST.get()) in
   let avail_in = get_avail_in ss in
   let len = if avail_in >^ size then
     size
   else
     avail_in
   in
-  let avail_in' = B.sub ss 0ul 1ul in
   let next_in' = !*next_in in
   let ulen = Ghost.hide (Seq.length block_data) in
     
-  B.blit (CB.cast next_in') 0ul buf 0ul len;
+  B.blit (CB.cast next_in') 0ul window from len;
+  let h1 = Ghost.hide (ST.get ()) in
   let buf' = CB.sub next_in' 0ul (Ghost.hide len) in
   if wrap = 1l then
     set_adler ss (Adler32.adler32 #ulen (Ghost.reveal block_data) (get_adler ss) buf' len)
@@ -190,98 +167,139 @@ inline_for_extraction let read_buf
   next_in *= (CB.sub next_in' len (avail_in -^ len));
   set_avail_in ss (avail_in -^ len);
   set_total_in ss (U32.add_underspec (get_total_in ss) len);
-  (len, Ghost.hide buf')
 
-let w_size_fit_u32 (w_size: U32.t{U32.v w_size < pow2 15}): Lemma
-  (ensures 2 * U32.v w_size < pow2 32)
-  [SMTPat (2 * U32.v w_size)] = 
-  Math.pow2_double_mult 15
+  let h1 = Ghost.hide (ST.get ()) in
+  let w0 = Ghost.hide (B.as_seq h0 window) in
+  let w1 = Ghost.hide (B.as_seq h1 window) in
+  let block_data' = Ghost.hide (Seq.append block_data (CB.as_seq h1 buf')) in
+  let total_in = Ghost.hide (Seq.length block_data + v len)in
+  let w_len = Ghost.hide (v from + v len) in
+  assert(forall (i: nat{i < v from}).
+    let _1 = Seq.lemma_index_slice w0 0 (v from) i in
+    let _2 = Seq.lemma_index_slice w1 0 (v from) i in
+    (Seq.slice w0 0 (v from)).[i] == w0.[i] /\
+    (Seq.slice w1 0 (v from)).[i] == w1.[i] /\
+    (Seq.slice w0 0 (v from)).[i] == (Seq.slice w1 0 (v from)).[i]);
+  assert(forall (i: nat). i < v from ==> w0.[i] == w1.[i]);
 
-#set-options "--z3rlimit 2048 --fuel 0 --ifuel 0"
+  assert(forall (i: nat{v from < i /\ i < v from + v len}).
+    w1.[i] == block_data'.[total_in - w_len + i]);
+  
+  (len, block_data')
+
+inline_for_extraction
+let slide_index (buf: B.buffer U16.t) (offset i: U32.t):
+  ST.Stack unit
+  (requires fun h -> B.live h buf /\ U32.v i < B.length buf)
+  (ensures fun h0 _ h1 ->
+    let open U32 in
+    let value = U16.v (B.as_seq h0 buf).[v i] in
+    let value' = U16.v (B.as_seq h1 buf).[v i] in
+    (value > v offset ==> value' = value - v offset) /\
+    (value <= v offset ==> value' = 0) /\
+    B.modifies (B.loc_buffer buf) h0 h1 /\
+    LB.unchange_except h0 h1 buf (v i)) =
+  let open U32 in
+  let h0 = ST.get () in
+  let value = buf.(i) in
+  [@inline_let] let value' = Cast.uint16_to_uint32 value in
+  [@inline_let] let value'' =
+    Cast.uint32_to_uint16 (if value' >^ offset then value' -^ offset else 0ul)
+  in
+  buf.(i) <- value''
+
+#set-options "--z3rlimit 4096 --fuel 0 --ifuel 0 --z3seed 25 --z3refresh"
 [@@ CInline ]
-let rec slide_head (ctx: lz77_context_p) (h_size h_range: Ghost.erased U32.t) (i: U32.t):
+let rec slide_head
+  (ctx: lz77_context_p)
+  (state: lz77_state_t)
+  (h_size: Ghost.erased U32.t)
+  (i: U32.t):
   ST.Stack unit
   (requires fun h ->
-    S.context_valid h ctx /\
+    S.state_valid h ctx state /\
     (let ctx' = B.get h (CB.as_mbuf ctx) 0 in
     U32.v i <= U32.v ctx'.h_size /\
     U32.v h_size == U32.v ctx'.h_size /\
-    hash_range_pre_cond ctx' h_range /\
-    S.sub_head_valid h ctx h_range (fun j -> j >= U32.v i /\ j < U32.v ctx'.h_size) false /\
-    S.sub_head_valid h ctx h_range (fun j -> j < U32.v i) true))
+    S.sub_head_valid h ctx state (fun j -> j >= U32.v i /\ j < U32.v ctx'.h_size) false /\
+    S.sub_head_valid h ctx state (fun j -> j < U32.v i) true))
   (ensures fun h0 _ h1 ->
-    B.modifies (B.loc_buffer (B.get h0 (CB.as_mbuf ctx) 0).head) h0 h1 /\
-    S.head_valid h1 ctx h_range true)
+    let ctx' = B.get h0 (CB.as_mbuf ctx) 0 in
+    B.modifies (B.loc_buffer ctx'.head) h0 h1 /\
+    S.state_valid h1 ctx state /\
+    S.head_valid h1 ctx state true)
   (decreases U32.v h_size - U32.v i) =
   let open U32 in
+  let h0 = ST.get () in
   let head = (CB.index ctx 0ul).head in
   let w_size = (CB.index ctx 0ul).w_size in
   if i <^ (CB.index ctx 0ul).h_size then begin
-    let m = head.(i) in
-    [@inline_let] let m' = Cast.uint16_to_uint32 m in
-    head.(i) <- Cast.uint32_to_uint16 (if m' >=^ w_size then m' -^ w_size else 0ul);
-    slide_head ctx h_size h_range (i +^ 1ul)
+    slide_index head w_size i;
+
+    let h1 = Ghost.hide (ST.get ()) in
+    let ctx' = Ghost.hide (B.get h0 (CB.as_mbuf ctx) 0) in
+    assert(S.state_valid h1 ctx state);
+    assert(forall (i: nat). {:pattern (B.as_seq h1 (B.gsub ctx'.window ctx'.w_size ctx'.w_size)).[i]}
+      i < v ctx'.w_size ==>
+        (B.as_seq h1 (B.gsub ctx'.window ctx'.w_size ctx'.w_size)).[i] ==
+        (B.as_seq h1 ctx'.window).[i + v ctx'.w_size]);
+    assert(S.head_index_valid #h1 #ctx state true (v i));
+
+    slide_head ctx state h_size (i +^ 1ul)
   end else
     ()
 
-#set-options "--z3rlimit 2048 --fuel 0 --ifuel 0 --z3seed 25"
+#set-options "--z3rlimit 2048 --fuel 0 --ifuel 0 --z3seed 25 --z3refresh"
 [@ (CPrologue "#ifndef FASTEST")
    (CEpilogue "#endif")
    CInline]
-let rec slide_prev (ctx: lz77_context_p) (w_size h_range: Ghost.erased U32.t) (i: U32.t):
+let rec slide_prev
+  (ctx: lz77_context_p) (state: lz77_state_t) (w_size: Ghost.erased U32.t) (i: U32.t):
   ST.Stack unit
   (requires fun h ->
     let open U32 in
-    S.context_valid h ctx /\
+    S.state_valid h ctx state /\
     (let ctx' = B.get h (CB.as_mbuf ctx) 0 in
     CFlags.fastest == false /\
     U32.v i <= U32.v ctx'.w_size /\
     U32.v w_size == U32.v ctx'.w_size /\
-    hash_range_pre_cond ctx' h_range /\
-    S.sub_prev_valid h ctx h_range (fun j -> v i <= j /\ j < v w_size) false /\
-    S.sub_prev_valid h ctx h_range (fun j -> j < v i) true))
+    S.sub_prev_valid h ctx state (fun j -> v i <= j /\ j < v w_size) false /\
+    S.sub_prev_valid h ctx state (fun j -> j < v i) true))
   (ensures fun h0 _ h1 ->
     let open U32 in
-    S.context_valid h1 ctx /\
+    S.state_valid h1 ctx state /\
     B.modifies (B.loc_buffer (B.get h0 (CB.as_mbuf ctx) 0).prev) h0 h1 /\
-    hash_range_pre_cond (B.get h1 (CB.as_mbuf ctx) 0) h_range /\
-    S.prev_valid h1 ctx h_range true)
+    S.prev_valid h1 ctx state true)
   (decreases U32.v w_size - U32.v i) =
   let open U32 in
   let prev = (CB.index ctx 0ul).prev in
   let w_size' = (CB.index ctx 0ul).w_size in
   if i <^ w_size' then begin
-    let m = prev.(i) in
-    [@inline_let] let m' = Cast.uint16_to_uint32 m in
-    prev.(i) <- Cast.uint32_to_uint16 (if m' >=^ w_size' then m' -^ w_size' else 0ul);
-    let h = Ghost.hide (ST.get ()) in
-    assert(forall (j: nat{U32.v w_size <= j /\ j < U32.v h_range}).
-      let ctx' = Ghost.hide (B.get h (CB.as_mbuf ctx) 0) in
-      let window' = Ghost.hide (B.gsub ctx'.window w_size (h_range -^ w_size)) in
-      let s0 = B.as_seq h ctx'.window in
-      let s1 = B.as_seq h window' in
-      s0.[j] == s1.[j - U32.v w_size]);
-    slide_prev ctx w_size h_range (i +^ 1ul)
+    slide_index prev w_size' i;
+    slide_prev ctx state w_size (i +^ 1ul)
   end else
     ()
 
-let slide_hash ctx h_range =
+let slide_hash ctx state =
   ST.push_frame ();
   let open U32 in
+  let head = (CB.index ctx 0ul).head in
   let w_size = (CB.index ctx 0ul).w_size in
   let h_size = (CB.index ctx 0ul).h_size in
-  if CFlags.fastest then
-    if h_range >^ w_size then begin
-      slide_head ctx h_size h_range 0ul;
-      let h = ST.get () in assert(S.head_valid h ctx h_range true)
-    end else
-      clear_hash ctx
-  else
-    if h_range >^ w_size then begin
-      slide_head ctx h_size h_range 0ul;
-      slide_prev ctx w_size h_range 0ul
-    end else
-      clear_hash ctx;
+  let h_range = get_strstart state -^ get_insert state in
+  if h_range >^ w_size then
+    if CFlags.fastest then
+      slide_head ctx state h_size 0ul
+    else begin
+      slide_head ctx state h_size 0ul;
+      slide_prev ctx state w_size 0ul
+    end
+  else begin
+    B.fill (CB.index ctx 0ul).head 0us h_size;
+    let h1 = Ghost.hide (ST.get ()) in
+    assert(Seq.equal (Seq.slice (B.as_seq h1 head) 0 (v h_size)) (B.as_seq h1 head));
+    assert(forall (i: nat). i < v h_size ==> U16.v (B.as_seq h1 head).[i] == 0)
+  end;
   ST.pop_frame ()
 
 [@@ CInline ]
@@ -290,68 +308,50 @@ let slide_window_buf
   (ctx: lz77_context_p)
   (state: lz77_state_t)
   (block_start: B.pointer I32.t)
-  (len: U32.t):
+  (block_data: Ghost.erased (Seq.seq U8.t)):
   ST.Stack unit
   (requires fun h ->
-    S.slide_window_pre h ctx state block_start /\
-    U32.v len <= U32.v (B.get h (CB.as_mbuf ctx) 0).w_size)
-  (ensures fun h0 _ h1 ->
-    S.slide_window_buf_post h0 h1 ctx state block_start (U32.v len)) =
+    S.slide_window_pre h ctx state block_start block_data /\
+    S.strstart (B.as_seq h state) >= U32.v (B.get h (CB.as_mbuf ctx) 0).w_size)
+  (ensures fun h0 _ h1 -> S.slide_window_buf_post h0 h1 ctx state block_start block_data) =
   let open U32 in
   let w_size = (CB.index ctx 0ul).w_size in
-  let w_size' = Ghost.hide (U32.v w_size) in
   let window = (CB.index ctx 0ul).window in
   let w_bits = Ghost.hide (CB.index ctx 0ul).w_bits in
-  S.window_size_upper_bound (U16.v w_bits) (v w_size);
+  
   let left = B.sub window 0ul w_size in
   let right = B.sub window w_size w_size in
   let h0 = Ghost.hide (ST.get ()) in
   let ctx' = Ghost.hide (B.get h0 (CB.as_mbuf ctx) 0) in
   let w0 = Ghost.hide (B.as_seq h0 ctx'.window) in
   
+  let len = get_lookahead state +^ get_strstart state -^ w_size in
   B.blit right 0ul left 0ul len;
+
   set_match_start (U16.v w_bits) (v w_size) state ((get_match_start state) -^ w_size);
   set_strstart (U16.v w_bits) (v w_size) state ((get_strstart state) -^ w_size);
+
+  if get_insert state >^ get_strstart state then
+    set_insert state (get_strstart state)
+  else
+    ();
   block_start *= I32.sub (!*block_start) (Cast.uint32_to_int32 w_size);
   let h1 = Ghost.hide (ST.get ()) in
   let w1 = Ghost.hide (B.as_seq h1 ctx'.window) in
+  let w_end0 = Ghost.hide (S.window_end (B.as_seq h0 state)) in
+  let w_end1 = Ghost.hide (S.window_end (B.as_seq h1 state)) in
   assert(forall (i: nat{i < U32.v len}).
-    (B.as_seq h0 (B.gsub ctx'.window ctx'.w_size len)).[i] == w0.[i + w_size'] /\
+    (B.as_seq h0 (B.gsub ctx'.window ctx'.w_size len)).[i] == w0.[i + v w_size] /\
     (B.as_seq h1 (B.gsub ctx'.window 0ul len)).[i] ==
     (B.as_seq h0 (B.gsub ctx'.window ctx'.w_size len)).[i] /\
     (B.as_seq h1 (B.gsub ctx'.window 0ul len)).[i] == w1.[i]);
-  assert(forall (i: nat{i < U32.v len}). w0.[i + w_size'] == w1.[i])
-
-#set-options "--z3rlimit 4096 --fuel 0 --ifuel 0"
-[@@ CInline ]
-inline_for_extraction
-let slide_window
-  (ctx: lz77_context_p)
-  (state: lz77_state_t)
-  (block_start: B.pointer I32.t):
-  ST.StackInline U32.t
-  (requires fun h ->
-    let open U32 in
-    let state' = B.as_seq h state in
-    S.slide_window_pre h ctx state block_start /\
-    S.hash_chain_valid h ctx (U32.uint_to_t (S.hash_end state')) false)
-  (ensures fun h0 more h1 -> S.slide_window_post h0 more h1 ctx state block_start) =
-  let open U32 in
-  let h0 = Ghost.hide (ST.get ()) in
-  let strstart = get_strstart state in
-  let w_size = (CB.index ctx 0ul).w_size in
-  let h_range = strstart -^ get_insert state in
-  let window = Ghost.hide (CB.index ctx 0ul).window in
-  let more = (CB.index ctx 0ul).window_size -^ get_lookahead state -^ strstart in
-  if strstart >=^ w_size then begin
-    slide_hash ctx h_range;
-    slide_window_buf ctx state block_start (w_size -^ more);
-    let h1 = Ghost.hide (ST.get ()) in
-    LB.as_seq_gsub_eq h0 h1 window window
-      w_size 0ul (w_size -^ more) (h_range -^ w_size +^ (min_match -^ 1ul));
-    more +^ w_size
-  end else
-    more
+  assert(forall i. {:pattern (w1.[i])} i < v len ==>
+    w0.[i + v w_size] == w1.[i] /\
+    w0.[i + v w_size] == block_data.[Seq.length block_data - w_end1 + i]);
+  assert(forall i.{:pattern (block_data.[Seq.length block_data - w_end1 + i])} i < v len ==>
+    w1.[i] == block_data.[Seq.length block_data - w_end1 + i]);
+  assert(forall i. {:pattern (w1.[i])} i < v len ==>
+    (B.as_seq h0 (B.gsub window w_size w_size)).[i] == w1.[i])
 
 inline_for_extraction
 let min_lookahead (ctx: lz77_context_p):
@@ -360,9 +360,34 @@ let min_lookahead (ctx: lz77_context_p):
   (ensures fun h0 res h1 ->
     B.modifies B.loc_none h0 h1 /\
     U32.v res = S.min_lookahead (B.get h1 (CB.as_mbuf ctx) 0)) =
-  if (CB.index ctx 0ul).w_bits = 8us then 256ul else 258ul
+  if (CB.index ctx 0ul).w_bits = 8us then 128ul else 258ul
 
-#set-options "--z3rlimit 8192 --fuel 0 --ifuel 1 --z3seed 13"
+#set-options "--z3rlimit 4096 --fuel 0 --ifuel 0 --z3seed 1"
+[@@ CInline ]
+inline_for_extraction
+let slide_window
+  (ctx: lz77_context_p)
+  (state: lz77_state_t)
+  (block_start: B.pointer I32.t)
+  (block_data: Ghost.erased (Seq.seq U8.t)):
+  ST.Stack U32.t
+  (requires fun h ->
+    S.slide_window_pre h ctx state block_start block_data /\
+    S.hash_chain_valid h ctx state false)
+  (ensures fun h0 more h1 -> S.slide_window_post h0 more h1 ctx state block_start block_data) =
+  let open U32 in
+  let strstart = get_strstart state in
+  let w_size = (CB.index ctx 0ul).w_size in
+  let window_size = (CB.index ctx 0ul).window_size in
+  let more = (CB.index ctx 0ul).window_size -^ get_lookahead state -^ strstart in
+  if strstart >=^ window_size -^ min_lookahead ctx then begin
+    slide_hash ctx state;
+    slide_window_buf ctx state block_start block_data;
+    more +^ w_size
+  end else
+    more
+
+#set-options "--z3rlimit 32768 --fuel 0 --ifuel 0 --z3seed 7 --z3refresh"
 [@@ CInline ]
 let rec do_fill_window
   (ss:stream_state_t)
@@ -377,13 +402,11 @@ let rec do_fill_window
   (ensures fun h0 res h1 ->
     S.do_fill_window_post h0 res h1 ss ctx ls next_in wrap avail_in block_data)
   (decreases avail_in) =
-    let open U32 in let open FStar.Seq in
+    let open U32 in
     let h0 = Ghost.hide (ST.get ()) in
     let ctx' = Ghost.hide (B.get h0 (CB.as_mbuf ctx) 0) in
     let w_bits = Ghost.hide (U16.v ctx'.w_bits) in
     let w_size = Ghost.hide (v ctx'.w_size) in
-    S.window_size_lower_bound (U16.v ctx'.w_bits) (U32.v ctx'.w_size);
-    S.window_size_upper_bound (U16.v ctx'.w_bits) (U32.v ctx'.w_size);
     
     let window = (CB.index ctx 0ul).window in
     let window_size = (CB.index ctx 0ul).window_size in
@@ -391,61 +414,38 @@ let rec do_fill_window
     let strstart = get_strstart ls in
     
     let w_end = strstart +^ lookahead in
-    let w_end' = Ghost.hide (U32.v w_end) in
-    let w_left = Ghost.hide (B.gsub window 0ul w_end) in
     
     [@inline_let] let more = window_size -^ w_end in
-    let w_right= B.sub window w_end more in
 
-    let (len, rbuf) = read_buf ss block_data next_in w_right more wrap in
-    let h1 = Ghost.hide (ST.get ()) in
-    let rbuf' = Ghost.hide (CB.as_seq h0 rbuf) in
-    assert(forall (i: nat{i < S.hash_end (B.as_seq h0 ls) + S.min_match - 1}).
-      (B.as_seq h0 window).[i] == (B.as_seq h1 w_left).[i] /\
-      (B.as_seq h1 window).[i] == (B.as_seq h1 w_left).[i]);
-
-    let total_in = Ghost.hide (Seq.length block_data) in
-    let block_data' = Ghost.hide (block_data @| rbuf') in
-    assert(forall (i: nat{i < U32.v len}). 
-       (CB.as_seq h1 rbuf).[i] == (B.as_seq h1 window).[i + w_end']);
-    assert(forall (i: nat{i < w_end'}).
-      block_data.[total_in - w_end' + i] == (B.as_seq h1 w_left).[i] /\
-      (B.as_seq h1 w_left).[i] == (B.as_seq h1 window).[i]);
-    assert(forall (i: nat{i < w_end'}).
-      block_data.[total_in - w_end' + i] == (B.as_seq h1 window).[i]);
-    assert((forall (i: nat{i < Seq.length block_data}). {:pattern (block_data'.[i])}
-      block_data'.[i] == block_data.[i]));
+    let (len, block_data') =
+      read_buf ss block_data window window_size next_in w_end more wrap
+    in
     
     set_lookahead w_bits w_size ls (lookahead +^ len);
-    let lookahead' = get_lookahead ls in
-    let avail_in' = get_avail_in ss in
     init_input_hash ctx ls;
 
-    let min_lookahead = min_lookahead ctx in
-    S.min_lookahead_upper_bound h0 ctx;
-    
-    if lookahead' <^ min_lookahead && avail_in' >^ 0ul then
-      do_fill_window ss ctx ls next_in wrap (U32.v avail_in') (block_data @| rbuf')
-    else
-      Ghost.hide (block_data @| rbuf')
+    let lookahead' = get_lookahead ls in
+    let avail_in' = get_avail_in ss in
+    let ml = min_lookahead ctx in
 
-#set-options "--z3rlimit 8192 --fuel 0 --ifuel 0"
+    if lookahead' <^ ml && avail_in' >^ 0ul then
+      do_fill_window ss ctx ls next_in wrap (U32.v avail_in') block_data'
+    else
+      block_data'
+
+#set-options "--z3rlimit 65536 --fuel 0 --ifuel 0 --z3seed 13 --z3refresh"
 let fill_window ss ctx ls next_in wrap block_start block_data =
   let h0 = Ghost.hide (ST.get ()) in
   let ctx' = Ghost.hide (B.get h0 (CB.as_mbuf ctx) 0) in
-  S.window_size_upper_bound (U16.v ctx'.w_bits) (U32.v ctx'.w_size);
-  
-  ST.push_frame ();
+  let ls0 = Ghost.hide (B.as_seq h0 ls) in
   let open U32 in
-  let more = slide_window ctx ls block_start in
+
   let avail_in = get_avail_in ss in
-  let res = if avail_in>^ 0ul then
-    do_fill_window ss ctx ls next_in wrap (U32.v avail_in) block_data
-  else
+  if avail_in >^ 0ul then begin
+    let more = slide_window ctx ls block_start block_data in
+    do_fill_window ss ctx ls next_in wrap (v avail_in) block_data
+  end else
     block_data
-  in
-  ST.pop_frame ();
-  res
 
 [@ (CEpilogue "#include \"Yazi_LZ77_String.inc\"")]
 assume val ctz_compare:
@@ -555,7 +555,7 @@ unfold let slow_match_pre_cond
   (S.strstart s' < v ctx'.w_size ==> v limit == 0) /\
   v chain_length >= 1
 
-#set-options "--z3rlimit 4096 --fuel 0 --ifuel 0 --z3seed 13"
+#set-options "--z3rlimit 32768 --fuel 0 --ifuel 0 --z3seed 13 --z3refresh"
 [@ (CPrologue "#ifndef FASTEST")
    (CEpilogue "#endif")
    CInline]
@@ -597,7 +597,7 @@ let rec search_hash_chain
     let strstart' = Ghost.hide (U32.v strstart) in
     assert(forall (j: nat{j < S.min_match}).
       s1'.[j] == s2'.[j] /\ s1'.[j] == w.[strstart' + j] /\ s2'.[j] == w.[v i + j]);
-    assert(forall (j: nat{j < S.min_match}). {:pattern (w.[v i + j]); (w.[strstart' + j])}
+    assert(forall (j: nat{j < S.min_match}). {:pattern (w.[v i + j] == w.[strstart' + j])}
       w.[v i + j] == w.[strstart' + j]);
     (i, chain_length, true)
   end else if chain_length >^ 1ul then begin
@@ -637,7 +637,8 @@ let rec do_longest_match_slow
       v best_len >= S.min_match /\
       v cur_match < S.strstart s' /\
       S.strstart s' + v best_len <= S.window_end s' /\
-      (forall (i: nat{i < v best_len}). w.[v cur_match + i] == w.[S.strstart s' + i])))
+      (forall (i: nat{i < v best_len}). {:pattern (w.[v cur_match + i])}
+        w.[v cur_match + i] == w.[S.strstart s' + i])))
   (ensures fun h0 res h1 ->
     let open U32 in
     let ctx' = B.get h1 (CB.as_mbuf ctx) 0 in
@@ -652,6 +653,7 @@ let rec do_longest_match_slow
       (forall (i: nat{i < v bl}). w.[v cm + i] == w.[S.strstart s' + i])))
   (decreases U32.v chain_length) =
   let open U32 in
+  let h = Ghost.hide (ST.get ()) in
   let (cm, cl, cont) = search_hash_chain ctx s scan_end limit chain_length cur_match in
   if cont then begin
     let w_bits = (CB.index ctx 0ul).w_bits in
