code/Yazi.LZ77.fsti
@@ -12,25 +12,18 @@ module U8 = FStar.UInt8
 
 include Yazi.LZ77.Types
 
-private unfold let hash_range_pre_cond (ctx: lz77_context) (h_range: U32.t) =
-  let open FStar.Mul in
-  U32.v ctx.w_size < U32.v h_range /\ U32.v h_range <= U32.v ctx.window_size - S.min_match + 1
-
-val init_dict_hash: ctx: lz77_context_p -> state: lz77_state_t ->
+val init_input_hash: ctx: lz77_context_p -> state: lz77_state_t ->
   ST.Stack unit
-  (requires fun h -> S.init_dict_hash_pre h ctx state)
-  (ensures fun h0 _ h1 -> S.init_dict_hash_post h0 h1 ctx state)
+  (requires fun h -> S.init_input_hash_pre h ctx state)
+  (ensures fun h0 _ h1 -> S.init_input_hash_post h0 h1 ctx state)
 
-val slide_hash: ctx: lz77_context_p -> h_range: U32.t -> ST.Stack unit
+val slide_hash: ctx: lz77_context_p -> state: lz77_state_t -> ST.Stack unit
   (requires fun h ->
-    let open FStar.Mul in
-    S.context_valid h ctx /\
-    (let ctx' = B.get h (CB.as_mbuf ctx) 0 in
-    (U32.v ctx'.w_size == U32.v h_range \/ hash_range_pre_cond ctx' h_range) /\
-    S.hash_chain_valid h ctx h_range false))
+    S.state_valid h ctx state /\
+    S.hash_chain_valid h ctx state false)
   (ensures fun h0 _ h1 ->
     B.modifies (S.hash_loc_buffer h0 ctx) h0 h1 /\
-    S.hash_chain_valid h1 ctx h_range true)
+    S.hash_chain_valid h1 ctx state true)
 
 val fill_window:
     ss: SST.stream_state_t
@@ -43,7 +36,7 @@ val fill_window:
   -> ST.Stack (Ghost.erased (Seq.seq U8.t))
   (requires fun h -> S.fill_window_pre h ss ctx ls next_in wrap block_start block_data)
   (ensures fun h0 res h1 ->
-    S.fill_window_post h0 res h1 ss ctx ls next_in wrap block_start block_data)
+     S.fill_window_post h0 res h1 ss ctx ls next_in wrap block_start (Ghost.reveal block_data))
 
 val longest_match: ctx: lz77_context_p -> s: lz77_state_t -> cur_match: U32.t ->
   ST.Stack U32.t
